Better Module Functors without code duplication

Dataflow/Syntax.v
@@ -8,7 +8,7 @@ Open Scope list_scope.
 
 (** * The CoreDF dataflow language *)
 
-Module Type SYNTAX (Import Op : OPERATORS).
+Module Type PRE_SYNTAX (Import Op : OPERATORS).
   (** ** Clocks *)
 
   Inductive clock : Type :=
@@ -76,6 +76,12 @@ Module Type SYNTAX (Import Op : OPERATORS).
   Definition find_node (f : ident) : global -> option node :=
     List.find (fun n=> ident_eqb n.(n_name) f).
 
+End PRE_SYNTAX.
+
+Module Type SYNTAX (Import Op : OPERATORS).
+  
+  Include PRE_SYNTAX Op.
+
   (** ** Properties *)
 
   (** Stronger induction scheme for lexp *)
@@ -100,76 +106,6 @@ Module Type SYNTAX (Import Op : OPERATORS).
 
 End SYNTAX.
 
-Module SyntaxFun' (Import Op : OPERATORS).
-  (** ** Clocks *)
-
-  Inductive clock : Type :=
-  | Cbase : clock                          (* base clock *)
-  | Con : clock -> ident -> typ -> bool -> clock. (* subclock *)
-
-  Implicit Type ck : clock.
-
-  (** ** Expressions *)
-
-  Inductive lexp : Type :=
-  | Econst : val -> typ -> lexp
-  | Evar : ident -> typ -> lexp
-  | Ewhen : lexp -> ident -> bool -> lexp
-  | Eunop : unary_op -> lexp -> typ -> lexp
-  | Ebinop : binary_op -> lexp -> lexp -> typ -> lexp.
-
-  Fixpoint typeof (le: lexp): typ :=
-    match le with
-    | Econst _ ty
-    | Evar _ ty
-    | Eunop _ _ ty
-    | Ebinop _ _ _ ty => ty
-    | Ewhen e _ _ => typeof e
-    end.
-  
-  Definition lexps := nelist lexp.
-
-  Implicit Type le: lexp.
-  Implicit Type les: lexps.
-
-  (** ** Control expressions *)
-
-  Inductive cexp : Type :=
-  | Emerge : ident -> typ -> cexp -> cexp -> cexp 
-  | Eite : lexp -> cexp -> cexp -> cexp
-  | Eexp : lexp -> cexp.
-
-  Implicit Type ce: cexp.
-
-  (** ** Equations *)
-
-  Inductive equation : Type :=
-  | EqDef : ident -> clock -> cexp -> equation
-  | EqApp : ident -> clock -> ident -> lexps -> typ -> equation
-  | EqFby : ident -> clock -> val -> lexp -> equation.
-
-  Implicit Type eqn: equation.
-
-  (** ** Node *)
-
-  Record node : Type :=
-    mk_node {
-        n_name : ident;
-        n_input : nelist (ident * typ);
-        n_output : (ident * typ);
-        n_vars : list (ident * typ);
-        n_eqs : list equation }.
-
-  Implicit Type N: node.
-
-  (** ** Program *)
-
-  Definition global := list node.
-
-  Implicit Type G: global.
-
-  Definition find_node (f : ident) : global -> option node :=
-    List.find (fun n=> ident_eqb n.(n_name) f).
-  
-End SyntaxFun'.
-Module SyntaxFun <: SYNTAX := SyntaxFun'.
+Module SyntaxFun (Import Op : OPERATORS) <: SYNTAX Op.
+  Include PRE_SYNTAX Op.
+End SyntaxFun.
