DF2MP/Translation.v
@@ -33,7 +33,7 @@ Here, we take advantage of the fact that the result of a node
 application is assigned to a single variable. We use the name of that
 variable to identify the instance.  *)
 
-Module Type TRANSLATION
+Module Type PRE_TRANSLATION
        (Import Op: OPERATORS)
        (Import SynDF : Rustre.Dataflow.Syntax.SYNTAX Op)
        (Import SynMP : Rustre.Minimp.Syntax.SYNTAX Op).
@@ -157,119 +157,24 @@ Module Type TRANSLATION
     List.map translate_node G.
   (* =end= *)
 
-End TRANSLATION.
+End PRE_TRANSLATION.
 
-Module TranslationFun' (Import Op: OPERATORS)
+Module Type TRANSLATION
+       (Import Op: OPERATORS)
        (Import SynDF : Rustre.Dataflow.Syntax.SYNTAX Op)
        (Import SynMP : Rustre.Minimp.Syntax.SYNTAX Op).
 
-  Definition gather_eq (acc: list (ident * typ) * list obj_dec) (eq: equation) :=
-    match eq with
-    | EqDef _ _ _     => acc
-    | EqApp x _ f _ _ => (fst acc, mk_obj_dec x f :: snd acc)
-    | EqFby x _ _ le  => ((x, SynDF.typeof le)::fst acc, snd acc)
-    end.
+  Include PRE_TRANSLATION Op SynDF SynMP. 
 
-  Definition gather_eqs (eqs: list equation) : (list (ident * typ) * list obj_dec) :=
-    List.fold_left gather_eq eqs ([], []).
+End TRANSLATION.
 
-  (** ** Translation *)
+Module TranslationFun
+       (Import Op: OPERATORS)
+       (Import SynDF : Rustre.Dataflow.Syntax.SYNTAX Op)
+       (Import SynMP : Rustre.Minimp.Syntax.SYNTAX Op)
+       <: TRANSLATION Op SynDF SynMP.
 
-  Section Translate.
-
-    Variable memories : PS.t.
-
-    (* =tovar= *)
-    Definition tovar (xt: ident * typ) : exp :=
-      let (x, ty) := xt in
-      if PS.mem x memories then State x ty else Var x ty.
-    (* =end= *)
-
-    (* =control= *)
-    Fixpoint Control (ck: clock) (s: stmt) : stmt :=
-      match ck with
-      | Cbase => s
-      | Con ck x ty true  => Control ck (Ifte (tovar (x, ty)) s Skip)
-      | Con ck x ty false => Control ck (Ifte (tovar (x, ty)) Skip s)
-      end.
-    (* =end= *)
-
-    (* =translate_lexp= *)
-    Fixpoint translate_lexp (e : lexp) : exp :=
-      match e with
-      | Econst c ty => Const c ty
-      | Evar x ty => tovar (x, ty)
-      | Ewhen e c x => translate_lexp e
-                                     (* | Eop op es => Op op (Nelist.map translate_lexp es) *)
-      | Eunop op e ty => Unop op (translate_lexp e) ty
-      | Ebinop op e1 e2 ty => Binop op (translate_lexp e1) (translate_lexp e2) ty
-      end.
-    (* =end= *)
-
-    (* =translate_cexp= *)
-    Fixpoint translate_cexp (x: ident) (e: cexp) : stmt :=
-      match e with
-      | Emerge y ty t f => Ifte (tovar (y, ty)) (translate_cexp x t) (translate_cexp x f)
-      | Eite b t f => Ifte (translate_lexp b) (translate_cexp x t) (translate_cexp x f)
-      | Eexp l => Assign x (translate_lexp l)
-      end.
-    (* =end= *)
-
-    (* =translate_eqn= *)
-    Definition translate_eqn (eqn: equation) : stmt :=
-      match eqn with
-      | EqDef x ck ce => Control ck (translate_cexp x ce)
-      | EqApp x ck f les ty => Control ck (Step_ap x ty f x (map translate_lexp les))
-      | EqFby x ck v le => Control ck (AssignSt x (translate_lexp le))
-      end.
-    (* =end= *)
-
-    (** Remark: eqns ordered in reverse order of execution for coherence with
-       [Is_well_sch]. *)
-
-    (* =translate_eqns= *)
-    Definition translate_eqns (eqns: list equation) : stmt :=
-      List.fold_left (fun i eq => Comp (translate_eqn eq) i) eqns Skip.
-    (* =end= *)
-
-  End Translate.
-
-  (* =translate_reset_eqn= *)
-  Definition translate_reset_eqn (s: stmt) (eqn: equation) : stmt :=
-    match eqn with
-    | EqDef _ _ _ => s
-    | EqFby x _ v0 _  => Comp (AssignSt x (Const v0 (typ_of_val v0))) s
-    | EqApp x _ f _ _ => Comp (Reset_ap f x) s
-    end.
-  (* =end= *)
-
-  (* =translate_reset_eqns= *)
-  Definition translate_reset_eqns (eqns: list equation): stmt :=
-    List.fold_left translate_reset_eqn eqns Skip.
-  (* =end= *)
-
-  Definition ps_from_list (l: list ident) : PS.t :=
-    List.fold_left (fun s i=>PS.add i s) l PS.empty.
-
-  (* =translate_node= *)
-  Definition translate_node (n: node): class :=
-    let names := gather_eqs n.(n_eqs) in
-    let mems := ps_from_list (List.map (@fst ident typ) (fst names)) in
-    mk_class n.(n_name)
-             n.(n_input)
-             n.(n_output)
-             n.(n_vars)
-             (fst names)
-             (snd names)
-             (translate_eqns mems n.(n_eqs))
-             (translate_reset_eqns n.(n_eqs)).
-  (* =end= *)
-
-  (* =translate= *)
-  Definition translate (G: global) : program :=
-    List.map translate_node G.
-  (* =end= *)
-
+  Include PRE_TRANSLATION Op SynDF SynMP. 
 
   (* (** ** Properties *) *)
 
@@ -297,5 +202,4 @@ Module TranslationFun' (Import Op: OPERATORS)
   (* Qed. *)
 
   
-End TranslationFun'.
-Module TranslationFun <: TRANSLATION := TranslationFun'.
+End TranslationFun.
