Dataflow/IsDefined.v
@@ -17,7 +17,7 @@ Require Import Rustre.Dataflow.Memories.
 
  *)
 
-Module Type ISDEFINED
+Module Type PRE_ISDEFINED
        (Op : OPERATORS)
        (Import Syn : SYNTAX Op)
        (Import Mem : MEMORIES Op Syn).
@@ -31,6 +31,15 @@ Module Type ISDEFINED
   Definition Is_defined_in_eqs (x: ident) (eqs: list equation) : Prop :=
     List.Exists (Is_defined_in_eq x) eqs.
 
+End PRE_ISDEFINED.
+
+Module Type ISDEFINED
+       (Op : OPERATORS)
+       (Import Syn : SYNTAX Op)
+       (Import Mem : MEMORIES Op Syn).
+
+  Include PRE_ISDEFINED Op Syn Mem.
+  
   Axiom Is_defined_in_eq_dec:
     forall x eq, {Is_defined_in_eq x eq}+{~Is_defined_in_eq x eq}.
 
@@ -65,19 +74,14 @@ Module Type ISDEFINED
 
 End ISDEFINED.
 
-Module IsDefinedFun'
+Module IsDefinedFun
        (Op : OPERATORS)
        (Import Syn : SYNTAX Op)
-       (Import Mem : MEMORIES Op Syn).
+       (Import Mem : MEMORIES Op Syn)
+       <: ISDEFINED Op Syn Mem.
 
-  Inductive Is_defined_in_eq : ident -> equation -> Prop :=
-  | DefEqDef: forall x ck e,      Is_defined_in_eq x (EqDef x ck e)
-  | DefEqApp: forall x ck f e ty, Is_defined_in_eq x (EqApp x ck f e ty)
-  | DefEqFby: forall x ck v e,    Is_defined_in_eq x (EqFby x ck v e).
-
-  Definition Is_defined_in_eqs (x: ident) (eqs: list equation) : Prop :=
-    List.Exists (Is_defined_in_eq x) eqs.
-
+  Include PRE_ISDEFINED Op Syn Mem.
+ 
   Lemma Is_defined_in_eq_dec:
     forall x eq, {Is_defined_in_eq x eq}+{~Is_defined_in_eq x eq}.
   Proof.
@@ -179,6 +183,4 @@ Module IsDefinedFun'
         apply In_memory_eq_Is_defined_eq in HH; auto.
   Qed.
 
-End IsDefinedFun'.
-
-Module IsDefinedFun <: ISDEFINED := IsDefinedFun'.
+End IsDefinedFun.
